@prefix : <http://rdf.geohistoricaldata.org/def/address#> .
@base <http://rdf.geohistoricaldata.org/def/address#> .

#Others namespaces
@prefix owl: <http://www.w3.org/2002/07/owl#> .
@prefix rdf: <http://www.w3.org/1999/02/22-rdf-syntax-ns#> .
@prefix xml: <http://www.w3.org/XML/1998/namespace> .
@prefix xsd: <http://www.w3.org/2001/XMLSchema#> .
@prefix prov: <http://www.w3.org/ns/prov#> .
@prefix rdfs: <http://www.w3.org/2000/01/rdf-schema#> .
@prefix skos: <http://www.w3.org/2004/02/skos/core#> .
@prefix time: <http://www.w3.org/2006/time#> .
@prefix voaf: <http://purl.org/vocommons/voaf#> .
@prefix organization: <http://www.w3.org/ns/org#> .
@prefix vann: <http://purl.org/vocab/vann/> .
@prefix dcterms: <http://purl.org/dc/terms/> .
@prefix cc: <http://creativecommons.org/ns#> .

# Core namespaces
@prefix atype: <http://rdf.geohistoricaldata.org/id/codes/address/attributeType/> .
@prefix ctype: <http://rdf.geohistoricaldata.org/id/codes/address/changeType/> .
@prefix ltype: <http://rdf.geohistoricaldata.org/id/codes/address/landmarkType/> .
@prefix lrtype: <http://rdf.geohistoricaldata.org/id/codes/address/landmarkRelationType/> .

<http://rdf.geohistoricaldata.org/def/address> rdf:type owl:Ontology .

#################################################################
#    Ontology metadata
#################################################################

<http://rdf.geohistoricaldata.org/def/cadastre#> a owl:Ontology, voaf:Vocabulary ;
        dcterms:creator [
	      a foaf:Person ;
	      organization:hasMembership [
	          a organization:Membership ;
	          organization:memberDuring [
	              a time:Interval ;
	              time:hasBeginning [
	                  a time:Instant ;
	                  time:inXSDDateTimeStamp "2019-10-15"^^xsd:dateTimeStamp ;
	                ] ;
	            ] ;
	          organization:organization <http://www.ign.fr/> ;
	          organization:organization <http://www.umr-lastig.fr/> ;
	          organization:role [
	              a organization:Role ;
	              rdfs:label "Doctorant"@fr, "PhD Student"@en ;
	            ] ;
	        ] ;
	      foaf:family_name "Bernard" ;
	      foaf:firstName "Charly" ;
	      foaf:mbox <mailto:charly.bernard@ign.fr> ;
	      foaf:name "Charly Bernard" ;
          foaf:workInfoHomepage <https://www.umr-lastig.fr/charly-bernard/> ;
	    ] ;
        dcterms:description "Ontologie PeGaZus pour décrire l'évolution des entités géographiques"@fr,
		                    "PeGaZus ontology to describe evolution of geographical entities"@en;
        dcterms:issued "2023-10-30"^^xsd:date ;
        dcterms:modified "2024-09-13"^^xsd:date ;
        dcterms:publisher <http://fr.dbpedia.org/resource/Institut_national_de_l%27information_g%C3%A9ographique_et_foresti%C3%A8re> ;
        dcterms:title "Ontologie PeGaZus"@fr, "PeGaZus ontology"@en ;
        vann:preferredNamespacePrefix "addr" ;
		vann:preferredNamespaceUri <http://rdf.geohistoricaldata.org/def/address#> ;
		dcterms:rights "Copyright 2024, IGN" ;
		cc:license <http://www.data.gouv.fr/Licence-Ouverte-Open-Licence> ;
		cc:license <http://creativecommons.org/licenses/by/2.0/> ;
		cc:license <http://opendatacommons.org/licenses/by/> ;
    #owl:priorVersion <> ;
		owl:versionInfo "Version 0.1 - 2024-09-13" .

#################################################################
#    Annotation properties
#################################################################

###  http://www.w3.org/2002/07/owl#maxQualifiedCardinality
owl:maxQualifiedCardinality rdf:type owl:AnnotationProperty .


###  http://www.w3.org/2004/02/skos/core#altLabel
skos:altLabel rdf:type owl:AnnotationProperty .


###  http://www.w3.org/2004/02/skos/core#broader
skos:broader rdf:type owl:AnnotationProperty .


###  http://www.w3.org/2004/02/skos/core#definition
skos:definition rdf:type owl:AnnotationProperty .


###  http://www.w3.org/2004/02/skos/core#inScheme
skos:inScheme rdf:type owl:AnnotationProperty .


###  http://www.w3.org/2004/02/skos/core#prefLabel
skos:prefLabel rdf:type owl:AnnotationProperty .


#################################################################
#    Object Properties
#################################################################

###  http://rdf.geohistoricaldata.org/def/address#hasNextVersion
:hasNextVersion rdf:type owl:ObjectProperty ;
       owl:inverseOf :hasPreviousVersion ;
       rdfs:comment "Décrit qu'une version de repère en précède une autre"@fr, "Describes that one landmark version precedes another"@en ;
       rdfs:label "a pour version suivante"@fr, "has next version"@en .

###  http://rdf.geohistoricaldata.org/def/address#hasPreviousVersion
:hasPreviousVersion rdf:type owl:ObjectProperty ;
      owl:inverseOf :hasNextVersion ;
      rdfs:comment "Décrit qu'une version de repère en succède à une autre"@fr, "Describes that one landmark version follows another"@en ;
      rdfs:label "a pour version précédente"@fr, 'has previous version'@en .

###  http://rdf.geohistoricaldata.org/def/address#hasOverlappingVersion
:hasOverlappingVersion rdf:type owl:ObjectProperty ;
      owl:inverseOf :isOverlappedByVersion ;
      rdfs:comment "Décrit qu'une version de repère en chevauche une autre"@fr, "Describes that one landmark version overlaps another"@en ;
      rdfs:label "chevauche la version"@fr, "overlaps version"@en .

###  http://rdf.geohistoricaldata.org/def/address#isOverlappedByVersion
:isOverlappedByVersion rdf:type owl:ObjectProperty ;
      owl:inverseOf :hasOverlappingVersion ;
      rdfs:comment "Décrit qu'une version de repère est chevauchée par une autre"@fr, "Describes that one landmark version is overlapped by another"@en ;
      rdfs:label "est chevauché par"@fr, "is overlapped by version"@en .

###  http://rdf.geohistoricaldata.org/def/address#hasTrace
addr:hasTrace a owl:ObjectProperty ;
    rdfs:label "a pour trace"@fr, "has trace"@en ;
    owl:inverseOf addr:isTraceOf.

###  http://rdf.geohistoricaldata.org/def/address#isTraceOf
addr:isTraceOf a owl:ObjectProperty ;
    rdfs:label "est une trace de"@fr, "is trace of"@en ;
    owl:inverseOf addr:hasTrace.

###  http://rdf.geohistoricaldata.org/def/address#hasRoot
:hasRoot rdf:type owl:ObjectProperty ;
       owl:inverseOf :isRootOf ;
       rdfs:comment "Décrit qu'un élément a pour racine un autre élement"@fr, "Describes that an element has another element of reference as its root"@en ;
       rdfs:label "a pour racine"@fr, "has root"@en .

###  http://rdf.geohistoricaldata.org/def/address#isRootOf
:isRootOf rdf:type owl:ObjectProperty ;
       owl:inverseOf :hasRoot ;
      rdfs:comment "Décrit qu'un élément est la racine d'un autre"@fr, "Describes that an element is the root of another"@en ;
      rdfs:label "est racine de"@fr, "is root of"@en .

###  http://rdf.geohistoricaldata.org/def/address#hasRootLandmark
:hasRootLandmark rdf:type owl:ObjectProperty ;
       rdfs:subPropertyOf :hasRoot ;
       owl:inverseOf :isRootLandmarkOf ;
       rdfs:comment "Décrit qu'un repère a pour racine un autre repère"@fr, "Describes that an landmark has another landmark as its root"@en ;
       rdfs:label "a pour racine"@fr, "has root"@en .

###  http://rdf.geohistoricaldata.org/def/address#isRootLandmarkOf
:isRootLandmarkOf rdf:type owl:ObjectProperty ;
       rdfs:subPropertyOf :isRootOf ;
      rdfs:comment "Décrit qu'un repère est la racine d'un autre"@fr, "Describes that an landmark is the root of another"@en ;
      rdfs:label "est racine de"@fr, "is root of"@en .

###  http://rdf.geohistoricaldata.org/def/address#appliedTo
:appliedTo rdf:type owl:ObjectProperty ;
           owl:inverseOf :changedBy ;
           rdfs:domain :Change ;
           rdfs:range [ rdf:type owl:Class ;
                        owl:unionOf ( :Attribute
                                      :Landmark
                                      :LandmarkRelation
                                    )
                      ] ;
           rdfs:comment "Définit sur quoi s'applique le changement"@fr, "Defines what the change applies to"@en ;
           rdfs:label "s'applique"@fr, "is applied to"@en .

###  http://rdf.geohistoricaldata.org/def/address#eventBefore
:eventBefore rdf:type owl:ObjectProperty ,
                owl:TransitiveProperty ;
       owl:inverseOf :eventAfter ;
       rdfs:domain :Event ;
       rdfs:range :Event ;
       rdfs:comment "Décrit la relation temporelle d'antériorité entre deux événéments"@fr, "Describes the temporal relationship of anteriority between two events"@en ;
       rdfs:label "est avant"@fr, "is before"@en .


###  http://rdf.geohistoricaldata.org/def/address#eventAfter
:eventAfter rdf:type owl:ObjectProperty ;
      owl:inverseOf :eventBefore ;
      rdf:type owl:TransitiveProperty ;
      rdfs:domain :Event ;
      rdfs:range :Event ;
      rdfs:comment "Décrit la relation temporelle de postériorité entre deux événements"@fr, "Describes the temporal relationship of posteriority between two events"@en ;
      rdfs:label "est après"@fr, "is after"@en .

###  http://rdf.geohistoricaldata.org/def/address#eventSameTime
:eventSameTime rdf:type owl:ObjectProperty ,
                   owl:SymmetricProperty ;
          rdfs:domain :Event ;
          rdfs:range :Event ;
          rdfs:comment "Décrit la relation temporelle de simultanéité entre deux événements"@fr, "Describes the temporal relationship of simultaneity between two events"@en ;
          rdfs:label "est en même temps que"@fr, "is at the same time"@en .

:instantBefore rdf:type owl:ObjectProperty ;
      owl:inverseOf :instantAfter ;
      rdf:type owl:TransitiveProperty ;
      rdfs:domain :CrispTimeInstant ;
      rdfs:range :CrispTimeInstant ;
      rdfs:comment "Décrit la relation temporelle d'antériorité entre deux instants"@fr, "Describes the temporal relationship of anteriority between two instants"@en ;
      rdfs:label "est avant"@fr, "is before"@en .

:instantAfter rdf:type owl:ObjectProperty ;
      owl:inverseOf :instantBefore ;
      rdf:type owl:TransitiveProperty ;
      rdfs:domain :CrispTimeInstant ;
      rdfs:range :CrispTimeInstant ;
      rdfs:comment "Décrit la relation temporelle de postériorité entre deux instants"@fr, "Describes the temporal relationship of posteriority between two instants"@en ;
      rdfs:label "est après"@fr, "is after"@en .

:instantSameTime rdf:type owl:ObjectProperty ;
      rdf:type owl:SymmetricProperty ;
      rdfs:domain :CrispTimeInstant ;
      rdfs:range :CrispTimeInstant ;
      rdfs:comment "Décrit la relation temporelle de simultanéité entre deux instants"@fr, "Describes the temporal relationship of simultaneity between two instants"@en ;
      rdfs:label "est en même temps que"@fr, "is at the same time"@en .

:instantMorePreciseThan rdf:type owl:ObjectProperty , owl:TransitiveProperty ;
      owl:inverseOf :instantLessPreciseThan ;
      rdfs:domain :CrispTimeInstant ;
      rdfs:range :CrispTimeInstant ;
      rdfs:comment "Compare les précisions temporelles entre deux instants"@fr, "Compares time accuracies between two instants"@en ;
      rdfs:label "est plus précis que"@fr, "is more precise than"@en .

:instantLessPreciseThan rdf:type owl:ObjectProperty , owl:TransitiveProperty ;
      owl:inverseOf :instantMorePreciseThan ;
      rdfs:domain :CrispTimeInstant ;
      rdfs:range :CrispTimeInstant ;
      rdfs:comment "Compare les précisions temporelles entre deux instants"@fr, "Compares time accuracies between two instants"@en ;
      rdfs:label "est moins précis que"@fr, "is less precise than"@en .

:instantAsPreciseAs rdf:type owl:ObjectProperty , owl:SymmetricProperty ;
      rdfs:domain :CrispTimeInstant ;
      rdfs:range :CrispTimeInstant ;
      rdfs:comment "Compare les précisions temporelles entre deux instants"@fr, "Compares time accuracies between two instants"@en ;
      rdfs:label "est aussi précis que"@fr, "is as precise as"@en .

time:after
  rdf:type owl:ObjectProperty ;
  rdfs:comment "Gives directionality to time. If a temporal entity T1 is after another temporal entity T2, then the beginning of T1 is after the end of T2."@en ;
  rdfs:domain time:TemporalEntity ;
  rdfs:label "after"@en ;
  rdfs:range time:TemporalEntity ;
  owl:inverseOf time:before ;
  skos:definition "Gives directionality to time. If a temporal entity T1 is after another temporal entity T2, then the beginning of T1 is after the end of T2."@en .

time:before
  rdf:type owl:ObjectProperty ;
  rdf:type owl:TransitiveProperty ;
  rdfs:comment "Gives directionality to time. If a temporal entity T1 is before another temporal entity T2, then the end of T1 is before the beginning of T2. Thus, \"before\" can be considered to be basic to instants and derived for intervals."@en ;
  rdfs:domain time:TemporalEntity ;
  rdfs:label "before"@en ;
  rdfs:range time:TemporalEntity ;
  owl:inverseOf time:after ;
  skos:definition "Gives directionality to time. If a temporal entity T1 is before another temporal entity T2, then the end of T1 is before the beginning of T2. Thus, \"before\" can be considered to be basic to instants and derived for intervals."@en .

time:intervalAfter
 rdf:type owl:ObjectProperty ;
 rdfs:comment "If a proper interval T1 is intervalAfter another proper interval T2, then the beginning of T1 is after the end of T2."@en ;
 rdfs:domain time:ProperInterval ;
 rdfs:label "interval after"@en ;
 rdfs:range time:ProperInterval ;
 rdfs:subPropertyOf time:after ;
 rdfs:subPropertyOf time:intervalDisjoint ;
 owl:inverseOf time:intervalBefore ;
 skos:definition "If a proper interval T1 is intervalAfter another proper interval T2, then the beginning of T1 is after the end of T2."@en .

time:intervalBefore
 rdf:type owl:ObjectProperty ;
 rdfs:comment "If a proper interval T1 is intervalBefore another proper interval T2, then the end of T1 is before the beginning of T2."@en ;
 rdfs:domain time:ProperInterval ;
 rdfs:label "interval before"@en ;
 rdfs:range time:ProperInterval ;
 rdfs:subPropertyOf time:before ;
 rdfs:subPropertyOf time:intervalDisjoint ;
 owl:inverseOf time:intervalAfter ;
 skos:definition "If a proper interval T1 is intervalBefore another proper interval T2, then the end of T1 is before the beginning of T2."@en .

time:intervalContains
 rdf:type owl:ObjectProperty ;
 rdfs:comment "If a proper interval T1 is intervalContains another proper interval T2, then the beginning of T1 is before the beginning of T2, and the end of T1 is after the end of T2."@en ;
 rdfs:domain time:ProperInterval ;
 rdfs:label "interval contains"@en ;
 rdfs:range time:ProperInterval ;
 owl:inverseOf time:intervalDuring ;
 skos:definition "If a proper interval T1 is intervalContains another proper interval T2, then the beginning of T1 is before the beginning of T2, and the end of T1 is after the end of T2."@en .

time:intervalDisjoint
 rdf:type owl:ObjectProperty ;
 rdfs:comment "If a proper interval T1 is intervalDisjoint another proper interval T2, then the beginning of T1 is after the end of T2, or the end of T1 is before the beginning of T2, i.e. the intervals do not overlap in any way, but their ordering relationship is not known."@en ;
 rdfs:domain time:ProperInterval ;
 rdfs:label "interval disjoint"@en ;
 rdfs:range time:ProperInterval ;
 skos:definition "If a proper interval T1 is intervalDisjoint another proper interval T2, then the beginning of T1 is after the end of T2, or the end of T1 is before the beginning of T2, i.e. the intervals do not overlap in any way, but their ordering relationship is not known."@en ;
 skos:note "This interval relation is not included in the 13 basic relationships defined in Allen (1984), but is defined in (T.3) as the union of time:intervalBefore v time:intervalAfter . However, that is outside OWL2 expressivity, so is implemented as an explicit property, with time:intervalBefore , time:intervalAfter as sub-properties"@en .

time:intervalDuring
 rdf:type owl:ObjectProperty ;
 rdfs:comment "If a proper interval T1 is intervalDuring another proper interval T2, then the beginning of T1 is after the beginning of T2, and the end of T1 is before the end of T2."@en ;
 rdfs:domain time:ProperInterval ;
 rdfs:label "interval during"@en ;
 rdfs:range time:ProperInterval ;
 rdfs:subPropertyOf time:intervalIn ;
 owl:inverseOf time:intervalContains ;
 skos:definition "If a proper interval T1 is intervalDuring another proper interval T2, then the beginning of T1 is after the beginning of T2, and the end of T1 is before the end of T2."@en .

time:intervalEquals
 rdf:type owl:ObjectProperty ;
 rdfs:comment "If a proper interval T1 is intervalEquals another proper interval T2, then the beginning of T1 is coincident with the beginning of T2, and the end of T1 is coincident with the end of T2."@en ;
 rdfs:domain time:ProperInterval ;
 rdfs:label "interval equals"@en ;
 rdfs:range time:ProperInterval ;
 owl:propertyDisjointWith time:intervalIn ;
 skos:definition "If a proper interval T1 is intervalEquals another proper interval T2, then the beginning of T1 is coincident with the beginning of T2, and the end of T1 is coincident with the end of T2."@en .

time:intervalFinishedBy
 rdf:type owl:ObjectProperty ;
 rdfs:comment "If a proper interval T1 is intervalFinishedBy another proper interval T2, then the beginning of T1 is before the beginning of T2, and the end of T1 is coincident with the end of T2."@en ;
 rdfs:domain time:ProperInterval ;
 rdfs:label "interval finished by"@en ;
 rdfs:range time:ProperInterval ;
 owl:inverseOf time:intervalFinishes ;
 skos:definition "If a proper interval T1 is intervalFinishedBy another proper interval T2, then the beginning of T1 is before the beginning of T2, and the end of T1 is coincident with the end of T2."@en .

time:intervalFinishes
 rdf:type owl:ObjectProperty ;
 rdfs:comment "If a proper interval T1 is intervalFinishes another proper interval T2, then the beginning of T1 is after the beginning of T2, and the end of T1 is coincident with the end of T2."@en ;
 rdfs:domain time:ProperInterval ;
 rdfs:label "interval finishes"@en ;
 rdfs:range time:ProperInterval ;
 rdfs:subPropertyOf time:intervalIn ;
 owl:inverseOf time:intervalFinishedBy ;
 skos:definition "If a proper interval T1 is intervalFinishes another proper interval T2, then the beginning of T1 is after the beginning of T2, and the end of T1 is coincident with the end of T2."@en .

time:intervalIn
 rdf:type owl:ObjectProperty ;
 rdfs:comment "If a proper interval T1 is intervalIn another proper interval T2, then the beginning of T1 is after the beginning of T2 or is coincident with the beginning of T2, and the end of T1 is before the end of T2, or is coincident with the end of T2, except that end of T1 may not be coincident with the end of T2 if the beginning of T1 is coincident with the beginning of T2."@en ;
 rdfs:domain time:ProperInterval ;
 rdfs:label "interval in"@en ;
 rdfs:range time:ProperInterval ;
 owl:propertyDisjointWith time:intervalEquals ;
 skos:definition "If a proper interval T1 is intervalIn another proper interval T2, then the beginning of T1 is after the beginning of T2 or is coincident with the beginning of T2, and the end of T1 is before the end of T2, or is coincident with the end of T2, except that end of T1 may not be coincident with the end of T2 if the beginning of T1 is coincident with the beginning of T2."@en ;
 skos:note "This interval relation is not included in the 13 basic relationships defined in Allen (1984), but is referred to as 'an important relationship' in Allen and Ferguson (1997). It is the disjoint union of time:intervalStarts v time:intervalDuring v time:intervalFinishes . However, that is outside OWL2 expressivity, so is implemented as an explicit property, with time:intervalStarts , time:intervalDuring , time:intervalFinishes as sub-properties"@en .

time:intervalMeets
 rdf:type owl:ObjectProperty ;
 rdfs:comment "If a proper interval T1 is intervalMeets another proper interval T2, then the end of T1 is coincident with the beginning of T2."@en ;
 rdfs:domain time:ProperInterval ;
 rdfs:label "interval meets"@en ;
 rdfs:range time:ProperInterval ;
 owl:inverseOf time:intervalMetBy ;
 skos:definition "If a proper interval T1 is intervalMeets another proper interval T2, then the end of T1 is coincident with the beginning of T2."@en .

time:intervalMetBy
 rdf:type owl:ObjectProperty ;
 rdfs:comment "If a proper interval T1 is intervalMetBy another proper interval T2, then the beginning of T1 is coincident with the end of T2."@en ;
 rdfs:domain time:ProperInterval ;
 rdfs:label "interval met by"@en ;
 rdfs:range time:ProperInterval ;
 owl:inverseOf time:intervalMeets ;
 skos:definition "If a proper interval T1 is intervalMetBy another proper interval T2, then the beginning of T1 is coincident with the end of T2."@en .

time:intervalOverlappedBy
 rdf:type owl:ObjectProperty ;
 rdfs:comment "If a proper interval T1 is intervalOverlappedBy another proper interval T2, then the beginning of T1 is after the beginning of T2, the beginning of T1 is before the end of T2, and the end of T1 is after the end of T2."@en ;
 rdfs:domain time:ProperInterval ;
 rdfs:label "interval overlapped by"@en ;
 rdfs:range time:ProperInterval ;
 owl:inverseOf time:intervalOverlaps ;
 skos:definition "If a proper interval T1 is intervalOverlappedBy another proper interval T2, then the beginning of T1 is after the beginning of T2, the beginning of T1 is before the end of T2, and the end of T1 is after the end of T2."@en .

time:intervalOverlaps
 rdf:type owl:ObjectProperty ;
 rdfs:comment "If a proper interval T1 is intervalOverlaps another proper interval T2, then the beginning of T1 is before the beginning of T2, the end of T1 is after the beginning of T2, and the end of T1 is before the end of T2."@en ;
 rdfs:domain time:ProperInterval ;
 rdfs:label "interval overlaps"@en ;
 rdfs:range time:ProperInterval ;
 owl:inverseOf time:intervalOverlappedBy ;
 skos:definition "If a proper interval T1 is intervalOverlaps another proper interval T2, then the beginning of T1 is before the beginning of T2, the end of T1 is after the beginning of T2, and the end of T1 is before the end of T2."@en .

time:intervalStartedBy
 rdf:type owl:ObjectProperty ;
 rdfs:comment "If a proper interval T1 is intervalStarted another proper interval T2, then the beginning of T1 is coincident with the beginning of T2, and the end of T1 is after the end of T2."@en ;
 rdfs:domain time:ProperInterval ;
 rdfs:label "interval started by"@en ;
 rdfs:range time:ProperInterval ;
 owl:inverseOf time:intervalStarts ;
 skos:definition "If a proper interval T1 is intervalStarted another proper interval T2, then the beginning of T1 is coincident with the beginning of T2, and the end of T1 is after the end of T2."@en .

time:intervalStarts
 rdf:type owl:ObjectProperty ;
 rdfs:comment "If a proper interval T1 is intervalStarts another proper interval T2, then the beginning of T1 is coincident with the beginning of T2, and the end of T1 is before the end of T2."@en ;
 rdfs:domain time:ProperInterval ;
 rdfs:label "interval starts"@en ;
 rdfs:range time:ProperInterval ;
 rdfs:subPropertyOf time:intervalIn ;
 owl:inverseOf time:intervalStartedBy ;
 skos:definition "If a proper interval T1 is intervalStarts another proper interval T2, then the beginning of T1 is coincident with the beginning of T2, and the end of T1 is before the end of T2."@en .

###  http://rdf.geohistoricaldata.org/def/address#changedBy
:changedBy rdf:type owl:ObjectProperty ;
           rdfs:domain [ rdf:type owl:Class ;
                         owl:unionOf ( :Attribute
                                       :Landmark
                                       :LandmarkRelation
                                     )
                       ] ;
           rdfs:range :Change ;
           rdfs:comment "Définit le changement qui est appliqué à l'élément"@fr, "Defines the change applied to the element"@en ;
           rdfs:label "changé par"@fr, "is changed by"@en .


###  http://rdf.geohistoricaldata.org/def/address#dependsOn
:dependsOn rdf:type owl:ObjectProperty ;
           owl:inverseOf :hasChange ;
           rdfs:domain :Change ;
           rdfs:range :Event ;
           rdfs:comment "Décrit l'appartenance d'un changement à un événement"@fr, "Describes whether a change belongs to an event"@en ;
           rdfs:label "dépend de l'événement"@fr, "depends on the event"@en .


###  http://rdf.geohistoricaldata.org/def/address#firstStep
:firstStep rdf:type owl:ObjectProperty ;
           rdfs:subPropertyOf :hasStep ;
           rdfs:domain :Address ;
           rdfs:range :AddressSegment ;
           rdfs:comment "Première étape de l'adresse."@fr, "First step of an address"@en ;
           rdfs:label "a pour première étape"@fr , "has first step"@en ;
           skos:altLabel "a pour premier segment d'adresse"@fr, "has as its first address segment"@en .


###  http://rdf.geohistoricaldata.org/def/address#hasAttribute
:hasAttribute rdf:type owl:ObjectProperty ;
              owl:inverseOf :isAttributeOf ;
              rdfs:domain owl:Thing ;
              rdfs:range :Attribute ;
              rdfs:comment "Décrit l'attribut pour un élement"@fr, "Describes the attribute for an element"@en ;
              rdfs:label "a pour attribut"@fr , "has attribute"@en.


###  http://rdf.geohistoricaldata.org/def/address#hasAttributeVersion
:hasAttributeVersion rdf:type owl:ObjectProperty ;
                     owl:inverseOf :isAttributeVersionOf ;
                     rdfs:domain :Attribute ;
                     rdfs:range :AttributeVersion ;
                     rdfs:comment "Version d'une valeur associée à l'attribut"@fr, "Version of a value associated with the attribute"@en ;
                     rdfs:label "a pour version"@fr, "has version"@en.


###  http://rdf.geohistoricaldata.org/def/address#hasBeginning
:hasBeginning rdf:type owl:ObjectProperty ;
              rdfs:domain :TimeInterval ;
              rdfs:range :TimeInstant ;
              rdfs:comment "Début de l'intervalle temporel"@fr, "Start of time interval"@en ;
              rdfs:label "commence par"@fr, "has beginning"@en .


###  http://rdf.geohistoricaldata.org/def/address#hasChange
:hasChange rdf:type owl:ObjectProperty ;
           rdfs:domain :Event ;
           rdfs:range :Change ;
           rdfs:comment "Définit les changements qui sont liés à l'événement"@fr, "Defines the changes linked to the event"@en ;
           rdfs:label "comporte le changement"@fr ,
                      "has change"@en .


###  http://rdf.geohistoricaldata.org/def/address#hasEnd
:hasEnd rdf:type owl:ObjectProperty ;
        rdfs:domain :TimeInterval ;
        rdfs:range :TimeInstant ;
        rdfs:comment "Fin de l'intervalle temporel"@fr, "End of time interval"@en ;
        rdfs:label "finit par"@fr, "has end"@en .


###  http://rdf.geohistoricaldata.org/def/address#hasFuzzyBeggining
:hasFuzzyBeggining rdf:type owl:ObjectProperty ;
                   rdfs:domain :FuzzyTimeInstant ;
                   rdfs:range :CrispTimeInstant ;
                   rdfs:comment "Définit le début de validité pour un instant flou"@fr, "Defines the start of validity for a fuzzy instant"@en ;
                   rdfs:label "a pour début flou"@fr , "has fuzzy beginning"@en.


###  http://rdf.geohistoricaldata.org/def/address#hasFuzzyEnd
:hasFuzzyEnd rdf:type owl:ObjectProperty ;
             rdfs:domain :FuzzyTimeInstant ;
             rdfs:range :CrispTimeInstant ;
             rdfs:comment "Définit la fin de validité pour un instant flou"@fr, "Defines the end of validity for a fuzzy instant"@en ;
             rdfs:label "a pour fin floue"@fr , "has fuzzy end"@en.


###  http://rdf.geohistoricaldata.org/def/address#hasFuzzyPeak
:hasFuzzyPeak rdf:type owl:ObjectProperty ;
              rdfs:domain :FuzzyTimeInstant ;
              rdfs:range :CrispTimeInstant ;
              rdfs:comment "Définit le pic de validité pour un instant flou"@fr, "Defines the validity peak for a fuzzy instant"@en ;
              rdfs:label "a pour pic flou"@fr , "has fuzzy peak"@en.


###  http://rdf.geohistoricaldata.org/def/address#hasStep
:hasStep rdf:type owl:ObjectProperty ;
         owl:inverseOf :isStepOf ;
         rdf:type owl:TransitiveProperty ;
         rdfs:domain :Address ;
         rdfs:range :AddressSegment ;
         owl:propertyChainAxiom ( :firstStep
                                  :nextStep
                                ) ,
                                ( :hasStep
                                  :nextStep
                                ) ;
         rdfs:label "a pour étape"@fr ,
                    "has step"@en .


###  http://rdf.geohistoricaldata.org/def/address#hasTime
:hasTime rdf:type owl:ObjectProperty ;
         rdfs:range :TemporalEntity ;
         rdfs:comment "Valeur temporelle liée à une ressource"@fr, "Time value linked to a resource"@en ;
         rdfs:label "a pour valeur temporelle"@fr, "has time"@en .

###  http://rdf.geohistoricaldata.org/def/address#hasTimeAfter
:hasTimeAfter rdf:type owl:ObjectProperty ;
       rdfs:range :TemporalInstant ;
       rdfs:comment "Indique que la ressource est liée à un instant situé avant l'instant associé"@fr, "Indicates that the resource is linked to an instant prior to the associated instant"@en ;
       rdfs:label "se passe après"@fr, "occurs after"@en .

###  http://rdf.geohistoricaldata.org/def/address#hasTimeBefore
:hasTimeBefore rdf:type owl:ObjectProperty ;
       rdfs:range :TemporalInstant ;
       rdfs:comment "Indique que la ressource est liée à un instant situé après l'instant associé"@fr, "Indicates that the resource is linked to a time after the associated time"@en ;
       rdfs:label "se passe avant"@fr, "occurs before"@en .

###  http://rdf.geohistoricaldata.org/def/address#hasEarliestTimeInstant
:hasEarliestTimeInstant rdf:type owl:ObjectProperty ;
        rdfs:subPropertyOf :hasTimeAfter ;
        rdfs:range :TemporalInstant ;
        rdfs:comment "Instant au plus tôt lié à la ressource"@fr, "Earliest time linked to the resource"@en ;
        rdfs:label "instant au plus tôt"@fr, "has earliest time instant"@en .

###  http://rdf.geohistoricaldata.org/def/address#hasLatestTimeInstant
:hasLatestTimeInstant rdf:type owl:ObjectProperty ;
        rdfs:subPropertyOf :hasTimeBefore ;
        rdfs:range :TemporalInstant ;
        rdfs:comment "Instant au plus tard lié à la ressource"@fr, "Latest time linked to the resource"@en ;
        rdfs:label "instant au plus tard"@fr, "has latest time instant"@en .

###  http://rdf.geohistoricaldata.org/def/address#isAttributeOf
:isAttributeOf rdf:type owl:ObjectProperty ;
               owl:inverseOf :hasAttribute ;
               rdfs:comment "Définit le repère pour lequel l'attribut existe"@fr, "Defines the frame of reference for which the attribute exists"@en ;
               rdfs:label "est un attribut de"@fr, "is attribute of"@en .


###  http://rdf.geohistoricaldata.org/def/address#isAttributeType
:isAttributeType rdf:type owl:ObjectProperty ;
                 rdfs:domain :Attribute ;
                 rdfs:range :AttributeType ;
                 rdfs:comment "Décrit le type d'attribut."@fr, "Describes the type of attribute."@en ;
                 rdfs:label "est un attribut de type"@fr, "is attribute type"@en .


###  http://rdf.geohistoricaldata.org/def/address#isAttributeVersionOf
:isAttributeVersionOf rdf:type owl:ObjectProperty ;
                      rdfs:domain :AttributeVersion ;
                      rdfs:range :Attribute ;
                      rdfs:comment "Attribut associée à la version d'attribut"@fr, "Attribute associated with the attribute version"@en ;
                      rdfs:label "est une version de l'attribut"@fr, "is attribute version of"@en .


###  http://rdf.geohistoricaldata.org/def/address#isChangeType
:isChangeType rdf:type owl:ObjectProperty ;
              rdfs:domain :Change ;
              rdfs:range :ChangeType ;
              rdfs:comment "Décrit le type de changement."@fr, "Describes the type of change."@en ;
              rdfs:label "est une changement de type"@fr, "is change type"@en .


###  http://rdf.geohistoricaldata.org/def/address#isLandmarkRelationType
:isLandmarkRelationType rdf:type owl:ObjectProperty ;
                        rdfs:domain :LandmarkRelation ;
                        rdfs:range :LandmarkRelationType ;
                        rdfs:comment "Décrit le type de relation entre repères définie par la ressource."@fr, "Describes the type of landmark relation."@en ;
                        rdfs:label "est une relation entre repères de type"@fr, "is landmark relation type"@en .


###  http://rdf.geohistoricaldata.org/def/address#isLandmarkType
:isLandmarkType rdf:type owl:ObjectProperty ;
                rdfs:domain :Landmark ;
                rdfs:range :LandmarkType ;
                rdfs:comment "Décrit le type de repère définie par la ressource."@fr, "Describes the type of landmark."@en ;
                rdfs:label "est un repère de type"@fr ,
                           "is landmark type"@en .


###  http://rdf.geohistoricaldata.org/def/address#isStepOf
:isStepOf rdf:type owl:ObjectProperty ;
          rdfs:domain :AddressSegment ;
          rdfs:range :Address ;
          rdfs:label "est une étape de"@fr ,
                     "is a step of"@en .


###  http://rdf.geohistoricaldata.org/def/address#locatum
:locatum rdf:type owl:ObjectProperty ;
         rdfs:domain :LandmarkRelation ;
         rdfs:range :Landmark ;
         rdfs:comment "Donne le repère qui est le locatum pour la relation entre repères"@fr ,
                      "Gives the landmark which is the locatum for the landmark relation"@en ;
         rdfs:label "a pour locatum"@fr , "has locatum"@en .


###  http://rdf.geohistoricaldata.org/def/address#makesEffective
:makesEffective rdf:type owl:ObjectProperty ;
                owl:inverseOf :isMadeEffectiveBy ;
                rdfs:domain :AttributeChange ;
                rdfs:range :AttributeVersion ;
                rdfs:comment "Décrit le fait qu'un changement rend effectif une version d'un attribut"@fr, "Describes the fact that a change makes a version of an attribute effective"@en ;
                rdfs:label "rend effectif"@fr, "makes effective"@en .

###  http://rdf.geohistoricaldata.org/def/address#isMadeEffectiveBy
:isMadeEffectiveBy rdf:type owl:ObjectProperty ;
                owl:inverseOf :makesEffective ;
                rdfs:domain :AttributeVersion ;
                rdfs:range :AttributeChange ;
                rdfs:comment "Décrit le fait qu'une version d'un attribut est rendue effectif par un changement"@fr, "Describes the fact that a version of an attribute is made effective by a change"@en ;
                rdfs:label "est rendu effectif par"@fr, "is made effective by"@en .

###  http://rdf.geohistoricaldata.org/def/address#isOutdatedBy
:isOutdatedBy rdf:type owl:ObjectProperty ;
                owl:inverseOf :outdates ;
                rdfs:domain :AttributeVersion ;
                rdfs:range :AttributeChange ;
                rdfs:comment "Décrit le fait qu'une version d'un attribut est rendue caduc par un changement"@fr, "Describes the fact that a version of an attribute is rendered obsolete by a change"@en ;
                rdfs:label "est rendu caduc par"@fr, "is outdated by"@en .


###  http://rdf.geohistoricaldata.org/def/address#nextStep
:nextStep rdf:type owl:ObjectProperty ;
          rdfs:domain :AddressSegment ;
          rdfs:range :AddressSegment ;
          rdfs:label "a pour prochaine étape"@fr ,
                     "has next step"@en ;
          skos:altLabel "est suivi par"@fr ,
                        "is followed by"@en .


###  http://rdf.geohistoricaldata.org/def/address#outdates
:outdates rdf:type owl:ObjectProperty ;
          owl:inverseOf :isOutdatedBy ;
          rdfs:domain :AttributeChange ;
          rdfs:range :AttributeVersion ;
          rdfs:comment "Décrit le fait qu'un changement rend caduc une version d'un attribut"@fr, "Describes the fact that a change invalidates a version of an attribute"@en ;
          rdfs:label "rend caduc"@fr, "outdates"@en .


###  http://rdf.geohistoricaldata.org/def/address#relatum
:relatum rdf:type owl:ObjectProperty ;
         rdfs:domain :LandmarkRelation ;
         rdfs:range :Landmark ;
         rdfs:comment "Donne le repère qui est un des relatums pour la relation entre repères"@fr ,
                      "Gives the landmark which is one of the relatums for the landmark relation"@en ;
         rdfs:label "a pour relatum"@fr ,
                    "has relatum"@en .


###  http://rdf.geohistoricaldata.org/def/address#targets
:targets rdf:type owl:ObjectProperty ;
         rdfs:domain :Address ;
         rdfs:range :Landmark ;
         rdfs:comment "Cible le repère décrivant l'adresse."@fr, "Target the marker describing the address"@en ;
         rdfs:label "cible"@fr ,
                    "targets"@en .


###  http://rdf.geohistoricaldata.org/def/address#timeCalendar
:timeCalendar rdf:type owl:ObjectProperty ;
              rdfs:domain :CrispTimeInstant ;
              rdfs:range time:TRS ;
              rdfs:comment "Calendrier lié à l'instant (grégorien, julien, révolutionnaire)"@fr, "Time-based calendar (Gregorian, Julian, Revolutionary)"@en ;
              rdfs:label "a pour calendrier"@fr, "has calendar"@en .


###  http://rdf.geohistoricaldata.org/def/address#timePrecision
:timePrecision rdf:type owl:ObjectProperty ;
               rdfs:domain :CrispTimeInstant ;
               rdfs:range time:TemporalUnit ;
               rdfs:comment "Précision de l'instant (au jour, au mois, à l'année...)"@fr, "Time accuracy (to the day, month, year, etc.)"@en ;
               rdfs:label "a pour précision temporelle"@fr, "has time precision"@en .

###  http://rdf.geohistoricaldata.org/def/address#sameVersionValueAs
:sameVersionValueAs rdf:type owl:ObjectProperty , owl:SymmetricProperty ;
               rdfs:domain :AttributeVersion ;
               rdfs:range :AttributeVersion ;
               rdfs:comment "Indique que deux versions d'attributs ont des valeurs similaires"@fr, "Indicates that two versions of attributes have similar values"@en ;
               rdfs:label "a une valeur similaire à"@fr, "has same version value as"@en .

###  http://rdf.geohistoricaldata.org/def/address#differentVersionValueFrom
:differentVersionValueFrom rdf:type owl:ObjectProperty , owl:SymmetricProperty ;
              rdfs:domain :AttributeVersion ;
              rdfs:range :AttributeVersion ;
              rdfs:comment "Indique que deux versions d'attributs ont des valeurs différents"@fr, "Indicates that two versions of attributes have different values"@en ;
              rdfs:label "a une valeur différente de"@fr, "has different version value from"@en .

###  http://rdf.geohistoricaldata.org/def/address#versionOf
:versionOf rdf:type owl:ObjectProperty ;
           rdfs:domain :LandmarkVersion ;
           rdfs:range :Landmark ;
           rdfs:comment "Définit pour une version de quel repère elle dépend"@fr, "Defines which landmark a version depends on"@en ;
           rdfs:label "est une version de repère de"@fr, "is a version of"@en .


###  http://www.w3.org/ns/prov#wasDerivedFrom
prov:wasDerivedFrom rdf:type owl:ObjectProperty ;
                    rdfs:domain prov:Entity ;
                    rdfs:range prov:Entity ;
                    rdfs:comment "The more specific subproperties of prov:wasDerivedFrom (i.e., prov:wasQuotedFrom, prov:wasRevisionOf, prov:hadPrimarySource) should be used when applicable."@en ;
                    rdfs:isDefinedBy <http://www.w3.org/ns/prov-o#> ;
                    rdfs:label "est dérivé de"@fr ,
                               "was derived from"@en .

#################################################################
#    Data properties
#################################################################

###  http://rdf.geohistoricaldata.org/def/address#timeStamp
:timeStamp rdf:type owl:DatatypeProperty ;
           rdfs:domain :CrispTimeInstant ;
           rdfs:range xsd:dateTimeStamp ;
           rdfs:comment "Timestamp lié à l'instant"@fr ;
           rdfs:label "a pour timestamp"@fr .


###  http://rdf.geohistoricaldata.org/def/address#versionValue
:versionValue rdf:type owl:DatatypeProperty ;
              rdfs:domain :AttributeVersion ;
              rdfs:comment "Valeur de liée à une version d'attribut"@fr, "Value linked to an attribute version"@en ;
              rdfs:label "a pour valeur"@fr, "has version value"@en .


#################################################################
#    Classes
#################################################################

###  http://rdf.geohistoricaldata.org/def/address#Address
:Address rdf:type owl:Class ;
         rdfs:subClassOf [ rdf:type owl:Restriction ;
                           owl:onProperty :firstStep ;
                           owl:qualifiedCardinality "1"^^xsd:nonNegativeInteger ;
                           owl:onClass :AddressSegment
                         ] ,
                         [ rdf:type owl:Restriction ;
                           owl:onProperty :targets ;
                           owl:qualifiedCardinality "1"^^xsd:nonNegativeInteger ;
                           owl:onClass :Landmark
                         ] ;
         rdfs:label "address"@en ,
                    "adresse"@fr .


###  http://rdf.geohistoricaldata.org/def/address#AddressSegment
:AddressSegment rdf:type owl:Class ;
                rdfs:subClassOf :LandmarkRelation ,
                                [ rdf:type owl:Restriction ;
                                  owl:onProperty :relatum ;
                                  owl:minQualifiedCardinality "1"^^xsd:nonNegativeInteger ;
                                  owl:onClass :Landmark
                                ] ,
                                [ rdf:type owl:Restriction ;
                                  owl:onProperty :locatum ;
                                  owl:qualifiedCardinality "1"^^xsd:nonNegativeInteger ;
                                  owl:onClass :Landmark
                                ] ,
                                [ rdf:type owl:Restriction ;
                                  owl:onProperty :nextStep ;
                                  owl:maxQualifiedCardinality "1"^^xsd:nonNegativeInteger ;
                                  owl:onClass :AddressSegment
                                ] ;
                rdfs:label "address segment"@en ,
                           "segment d'adresse"@fr .


###  http://rdf.geohistoricaldata.org/def/address#Attribute
:Attribute rdf:type owl:Class ;
           rdfs:label "Attribut"@fr, "Attribute"@en .


###  http://rdf.geohistoricaldata.org/def/address#AttributeChange
:AttributeChange rdf:type owl:Class ;
                 rdfs:subClassOf :Change ;
                 rdfs:label "Change on an attribute"@en ,
                            "Changement sur l'attribut"@fr .


###  http://rdf.geohistoricaldata.org/def/address#AttributeType
:AttributeType rdf:type owl:Class ;
               rdfs:subClassOf skos:Concept ;
               rdfs:label "Type d'attribut"@fr, "attribute type"@en .


###  http://rdf.geohistoricaldata.org/def/address#AttributeVersion
:AttributeVersion rdf:type owl:Class ;
                  rdfs:label "Attribute version"@en ,
                             "Version de l'attribut"@fr .


###  http://rdf.geohistoricaldata.org/def/address#Change
:Change rdf:type owl:Class ;
        rdfs:subClassOf [ rdf:type owl:Restriction ;
                          owl:onProperty :appliedTo ;
                          owl:allValuesFrom [ rdf:type owl:Class ;
                                              owl:unionOf ( :Attribute
                                                            :Landmark
                                                            :LandmarkRelation
                                                          )
                                            ]
                        ] ;
        rdfs:label "Changement"@fr, "Change"@en .


###  http://rdf.geohistoricaldata.org/def/address#ChangeType
:ChangeType rdf:type owl:Class ;
            rdfs:subClassOf skos:Concept ;
            rdfs:label "Type de changement"@fr, "Change Type"@en .


###  http://rdf.geohistoricaldata.org/def/address#CrispTemporalEntity
:CrispTemporalEntity rdf:type owl:Class ;
                     rdfs:subClassOf :TemporalEntity ;
                     rdfs:label "Crisp temporal entity"@en ,
                                "Entité temporelle non floue"@fr .


###  http://rdf.geohistoricaldata.org/def/address#CrispTimeInstant
:CrispTimeInstant rdf:type owl:Class ;
                  rdfs:subClassOf :CrispTemporalEntity ,
                                  :TimeInstant ,
                                  [ rdf:type owl:Restriction ;
                                    owl:onProperty :timeCalendar ;
                                    owl:maxQualifiedCardinality "1"^^xsd:nonNegativeInteger ;
                                    owl:onClass time:TRS
                                  ] ,
                                  [ rdf:type owl:Restriction ;
                                    owl:onProperty :timePrecision ;
                                    owl:maxQualifiedCardinality "1"^^xsd:nonNegativeInteger ;
                                    owl:onClass time:TemporalUnit
                                  ] ,
                                  [ rdf:type owl:Restriction ;
                                    owl:onProperty :timeStamp ;
                                    owl:maxQualifiedCardinality "1"^^xsd:nonNegativeInteger ;
                                    owl:onDataRange xsd:dateTimeStamp
                                  ] ;
                  rdfs:label "Crisp time instant"@en ,
                             "Instant temporel précis"@fr .


###  http://rdf.geohistoricaldata.org/def/address#CrispTimeInterval
:CrispTimeInterval rdf:type owl:Class ;
                   rdfs:subClassOf :CrispTemporalEntity ,
                                   :TimeInterval ;
                   rdfs:label "Crisp time interval"@en ,
                              "Intervalle temporel précis"@fr .


###  http://rdf.geohistoricaldata.org/def/address#Event
:Event rdf:type owl:Class ;
       rdfs:comment "Événément décrivant une évolution impliquant une ou plusieurs ressources à un instant donné."@fr, "Event describing a development involving one or more resources at a given time."@en ;
       rdfs:label "Event"@en ,
                  "Événément"@fr .


###  http://rdf.geohistoricaldata.org/def/address#FinalAddressSegment
:FinalAddressSegment rdf:type owl:Class ;
                     rdfs:subClassOf :AddressSegment ,
                                     [ rdf:type owl:Restriction ;
                                       owl:onProperty :nextStep ;
                                       owl:cardinality "0"^^xsd:nonNegativeInteger
                                     ] ;
                     rdfs:label "final address segment"@en ,
                                "segment d'adresse final"@fr .


###  http://rdf.geohistoricaldata.org/def/address#FuzzyTemporalEntity
:FuzzyTemporalEntity rdf:type owl:Class ;
                     rdfs:subClassOf :TemporalEntity ;
                     rdfs:label "Entité temporelle floue"@fr ,
                                "Fuzzy temporal entity"@en .


###  http://rdf.geohistoricaldata.org/def/address#FuzzyTimeInstant
:FuzzyTimeInstant rdf:type owl:Class ;
                  rdfs:subClassOf :FuzzyTemporalEntity ,
                                  :TimeInstant ;
                  rdfs:label "Fuzzy time instant"@en ,
                             "Instant temporel flou"@fr .


###  http://rdf.geohistoricaldata.org/def/address#FuzzyTimeInterval
:FuzzyTimeInterval rdf:type owl:Class ;
                   rdfs:subClassOf :FuzzyTemporalEntity ,
                                   :TimeInterval ;
                   rdfs:label "Fuzzy time interval"@en ,
                              "Intervalle temporel flou"@fr .


###  http://rdf.geohistoricaldata.org/def/address#Landmark
:Landmark rdf:type owl:Class ;
          rdfs:label "Landmark"@en ,
                     "Repère"@fr ,
                     "Landmark"@en .


###  http://rdf.geohistoricaldata.org/def/address#LandmarkChange
:LandmarkChange rdf:type owl:Class ;
                rdfs:subClassOf :Change ;
                rdfs:label "Change on a landmark"@en ,
                           "Changement sur le repère"@fr .


###  http://rdf.geohistoricaldata.org/def/address#LandmarkRelation
:LandmarkRelation rdf:type owl:Class ;
                  rdfs:label "Landmark relation"@en ,
                             "Relation entre repères"@fr .


###  http://rdf.geohistoricaldata.org/def/address#LandmarkRelationChange
:LandmarkRelationChange rdf:type owl:Class ;
                        rdfs:subClassOf :Change ;
                        rdfs:label "Change on a landmark relation"@en ,
                                   "changement sur la relation entre repères"@fr .


###  http://rdf.geohistoricaldata.org/def/address#LandmarkRelationType
:LandmarkRelationType rdf:type owl:Class ;
                      rdfs:subClassOf skos:Concept ;
                      rdfs:label "type of landmark relation"@en ,
                                 "Type de relation entre repères"@fr .


###  http://rdf.geohistoricaldata.org/def/address#LandmarkType
:LandmarkType rdf:type owl:Class ;
              rdfs:subClassOf skos:Concept ;
              rdfs:label "Type de repère"@fr ,
                         "Type of landmark"@en .


###  http://rdf.geohistoricaldata.org/def/address#LandmarkVersion
:LandmarkVersion rdf:type owl:Class ;
                 rdfs:subClassOf [ rdf:type owl:Restriction ;
                                   owl:onProperty :hasTime ;
                                   owl:allValuesFrom :TimeInterval
                                 ] ;
                 rdfs:label "Landmark version"@en ,
                            "Version de repère"@fr .


###  http://rdf.geohistoricaldata.org/def/address#TemporalEntity
:TemporalEntity rdf:type owl:Class ;
                rdfs:subClassOf time:TemporalEntity ;
                rdfs:label "Entité temporelle"@fr ,
                           "Temporal entity"@en .


###  http://rdf.geohistoricaldata.org/def/address#TimeInstant
:TimeInstant rdf:type owl:Class ;
             rdfs:subClassOf :TemporalEntity ;
             rdfs:label "Instant"@fr ,
                        "Time instant"@en .


###  http://rdf.geohistoricaldata.org/def/address#TimeInterval
:TimeInterval rdf:type owl:Class ;
              rdfs:subClassOf :TemporalEntity ;
              rdfs:label "Intervalle temporel"@fr ,
                         "Time interval"@en .


###  http://www.w3.org/2004/02/skos/core#Concept
skos:Concept rdf:type owl:Class .


###  http://www.w3.org/2004/02/skos/core#ConceptScheme
skos:ConceptScheme rdf:type owl:Class .


###  http://www.w3.org/2006/time#TRS
time:TRS rdf:type owl:Class .


###  http://www.w3.org/2006/time#TemporalUnit
time:TemporalUnit rdf:type owl:Class .


###  http://www.w3.org/ns/prov#Entity
prov:Entity rdf:type owl:Class ;
            rdfs:isDefinedBy <http://www.w3.org/ns/prov-o#> ;
            rdfs:label "entité"@fr, "Entity"@en .


#################################################################
#    Individuals
#################################################################

###  http://rdf.geohistoricaldata.org/def/address#AttributeList
:AttributeList rdf:type owl:NamedIndividual ,
                        skos:ConceptScheme ;
               rdfs:comment "Liste des différents rôles pouvant être joués par un attribut, représentés comme une liste de concepts SKOS."@fr ;
               rdfs:label "Type d'attribut"@fr, "type of attribute"@en .


###  http://rdf.geohistoricaldata.org/def/address#ChangeList
:ChangeList rdf:type owl:NamedIndividual ,
                     skos:ConceptScheme ;
            rdfs:comment "Liste des différents rôles pouvant être joués par un changement, représentés comme une liste de concepts SKOS."@fr ;
            rdfs:label "Type de changement"@fr, "type of change"@en .


###  http://rdf.geohistoricaldata.org/def/address#LandmarkList
:LandmarkList rdf:type owl:NamedIndividual ,
                       skos:ConceptScheme ;
              rdfs:comment "Liste des différents rôles pouvant être joués par un repère, représentés comme une liste de concepts SKOS."@fr ;
              rdfs:label "Type de repère"@fr ,
                         "Type of landmark"@en .


###  http://rdf.geohistoricaldata.org/def/address#LandmarkRelationList
:LandmarkRelationList rdf:type owl:NamedIndividual ,
                               skos:ConceptScheme ;
                      rdfs:comment "Liste des différents rôles pouvant être joués par une relation entre repères, représentés comme une liste de concepts SKOS."@fr ;
                      rdfs:label "Type de relation entre repères"@fr ,
                                 "Type of landmark relation"@en .


###  http://rdf.geohistoricaldata.org/id/codes/address/attributeType/Geometry
atype:Geometry rdf:type owl:NamedIndividual ,
                        :AttributeType ,
                        skos:Concept ;
               skos:altLabel "Attribut de géométrie"@fr ,
                             "Geometry attribute"@en ;
               skos:definition "Attribut décrivant la géométrie d'un élément"@fr, "Attribute describing the geometry of an element"@en ;
               skos:inScheme :AttributeList ;
               skos:prefLabel "Geometry"@en ,
                              "Géométrie"@fr .


###  http://rdf.geohistoricaldata.org/id/codes/address/attributeType/InseeCode
atype:InseeCode rdf:type owl:NamedIndividual ,
                         :AttributeType ,
                         skos:Concept ;
                skos:altLabel "Attribut de code INSEE"@fr ,
                              "INSEE code"@en ;
                skos:definition "Attribut décrivant le code INSEE d'un élément"@fr, "Attribute describing the INSEE code of an element"@en ;
                skos:inScheme :AttributeList ;
                skos:prefLabel "Code INSEE"@fr ,
                               "INSEE code"@en .


###  http://rdf.geohistoricaldata.org/id/codes/address/attributeType/Name
atype:Name rdf:type owl:NamedIndividual ,
                    :AttributeType ,
                    skos:Concept ;
           skos:altLabel "Attribut de nom"@fr ,
                         "Name attribute"@en ;
           skos:definition "Attribut décrivant le nom d'un élément"@fr, "Attribute describing the name of an element"@en ;
           skos:inScheme :AttributeList ;
           skos:prefLabel "Name"@en ,
                          "Nom"@fr .


###  http://rdf.geohistoricaldata.org/id/codes/address/changeType/AttributeVersionAppearance
ctype:AttributeVersionAppearance rdf:type owl:NamedIndividual ,
                                          :ChangeType ,
                                          skos:Concept ;
                                 skos:definition "Changement décrivant l'apparition d'une version d'un attribut"@fr, "Change describing the appearance of a version of an attribute"@en ;
                                 skos:inScheme :ChangeList ;
                                 skos:prefLabel "Apparition d'une version d'un attribut"@fr ,
                                                "Appearance of an attribute version"@en .


###  http://rdf.geohistoricaldata.org/id/codes/address/changeType/AttributeVersionDisappearance
ctype:AttributeVersionDisappearance rdf:type owl:NamedIndividual ,
                                             :ChangeType ,
                                             skos:Concept ;
                                    skos:definition "Changement décrivant la disparition d'une version d'un attribut"@fr, "Change describing the disappearance of a version of an attribute"@en ;
                                    skos:inScheme :ChangeList ;
                                    skos:prefLabel "Disappearance of an attribute version"@en ,
                                                   "Disparition d'une version d'un attribut"@fr .


###  http://rdf.geohistoricaldata.org/id/codes/address/changeType/AttributeVersionTransition
ctype:AttributeVersionTransition rdf:type owl:NamedIndividual ,
                                          :ChangeType ,
                                          skos:Concept ;
                                 skos:definition "Changement décrivant la transition entre des versions (apparition et disparition) d'un attribut"@fr, "Change describing the transition between versions (appearance and disappearance) of an attribute"@en ;
                                 skos:inScheme :ChangeList ;
                                 skos:prefLabel "Transition between attribute versions"@en ,
                                                "Transition de versions d'un attribut"@fr .


###  http://rdf.geohistoricaldata.org/id/codes/address/changeType/LandmarkAppearance
ctype:LandmarkAppearance rdf:type owl:NamedIndividual ,
                                  :ChangeType ,
                                  skos:Concept ;
                         skos:definition "Changement décrivant l'apparition du repère"@fr, "Change describing the appearance of the landmark"@en ;
                         skos:inScheme :ChangeList ;
                         skos:prefLabel "Apparition du repère"@fr ,
                                        "Appearance of a landmark"@en .


###  http://rdf.geohistoricaldata.org/id/codes/address/changeType/LandmarkDisappearance
ctype:LandmarkDisappearance rdf:type owl:NamedIndividual ,
                                     :ChangeType ,
                                     skos:Concept ;
                            skos:definition "Changement décrivant la disparition du repère"@fr, "Change describing the disappearance of the landmark"@en ;
                            skos:inScheme :ChangeList ;
                            skos:prefLabel "Disappearance of a landmark"@en ,
                                           "Disparition du repère"@fr .


###  http://rdf.geohistoricaldata.org/id/codes/address/changeType/LandmarkRelationAppearance
ctype:LandmarkRelationAppearance rdf:type owl:NamedIndividual ,
                                          :ChangeType ,
                                          skos:Concept ;
                                 skos:definition "Changement décrivant l'apparition d'une relation entre repères."@fr, "Change describing the appearance of a landmark relation."@en ;
                                 skos:inScheme :ChangeList ;
                                 skos:prefLabel "Apparition de la relation entre repères"@fr ,
                                                "Appearance of a landmark relation"@en .


###  http://rdf.geohistoricaldata.org/id/codes/address/changeType/LandmarkRelationDisappearance
ctype:LandmarkRelationDisappearance rdf:type owl:NamedIndividual ,
                                             :ChangeType ,
                                             skos:Concept ;
                                    skos:definition "Changement décrivant la dissolution d'une relation entre repères."@fr, "Change describing the disappearance of a landmark relation."@en ;
                                    skos:inScheme :ChangeList ;
                                    skos:prefLabel "Disappearance of a landmark relation"@en ,
                                                   "Dissolution de la relation entre repères"@fr .


###  http://rdf.geohistoricaldata.org/id/codes/address/landmarkRelationType/Along
lrtype:Along rdf:type owl:NamedIndividual ,
                      :LandmarkRelationType ,
                      skos:Concept ;
             skos:definition "Relation entre repères définissant que le locatum longe le relatum"@fr, "Relation between landmarks defining that the locatum runs alongside the relatum"@en ;
             skos:inScheme :AdressSegmentList ;
             skos:prefLabel "Along"@en ,
                            "Le long de"@fr .

###  http://rdf.geohistoricaldata.org/id/codes/address/landmarkRelationType/Belongs
lrtype:Belongs rdf:type owl:NamedIndividual ,
                        :LandmarkRelationType ,
                        skos:Concept ;
               skos:definition "Relation entre des repères définissant que le locatum appartient au relatum"@fr, "Relation between landmarks defining that the locatum belongs to the relatum"@en ;
               skos:inScheme :LandmarkRelationList ;
               skos:prefLabel "Appartient à"@fr, "Belongs to"@en .


###  http://rdf.geohistoricaldata.org/id/codes/address/landmarkRelationType/Between
lrtype:Between rdf:type owl:NamedIndividual ,
                        :LandmarkRelationType ,
                        skos:Concept ;
               skos:definition "Relation entre repères définissant que le locatum est entre deux relatums"@fr, "Relation between landmarks defining that the locatum is between the relatums"@en ;
               skos:inScheme :AdressSegmentList ;
               skos:prefLabel "Between"@en ,
                              "Entre"@fr .


###  http://rdf.geohistoricaldata.org/id/codes/address/landmarkRelationType/Corner
lrtype:Corner rdf:type owl:NamedIndividual ,
                       :LandmarkRelationType ,
                       skos:Concept ;
              skos:definition "Relation entre repères définissant que le locatum est au coin du relatum"@fr, "Relation between landmarks defining that the locatum is at the corner the relatums"@en ;
              skos:inScheme :AdressSegmentList ;
              skos:prefLabel "Coin"@fr ,
                             "Corner"@en .


###  http://rdf.geohistoricaldata.org/id/codes/address/landmarkRelationType/IsPartOf
lrtype:IsPartOf rdf:type owl:NamedIndividual ,
                         :LandmarkRelationType ,
                         skos:Concept ;
                skos:definition "Relation entre repères définissant que le locatum fait partie du relatum"@fr, "Relation between landmarks defining that the locatum is part of the relatum"@en ;
                skos:inScheme :AdressSegmentList ;
                skos:prefLabel "Fait partie de"@fr ,
                               "Is part of"@en .


###  http://rdf.geohistoricaldata.org/id/codes/address/landmarkRelationType/IsSimilar
lrtype:IsSimilar rdf:type owl:NamedIndividual ,
                          :LandmarkRelationType ,
                          skos:Concept ;
                 skos:definition "Relation entre repères définissant que le locatum est la même chose que le relatum"@fr, "Relation between landmarks defining that the locatum is the same thing as the relatum"@en ;
                 skos:inScheme :AdressSegmentList ;
                 skos:prefLabel "Est similaire à"@fr ,
                                "Is similar as"@en .


###  http://rdf.geohistoricaldata.org/id/codes/address/landmarkRelationType/Touches
lrtype:Touches rdf:type owl:NamedIndividual ,
                        :LandmarkRelationType ,
                        skos:Concept ;
               skos:altLabel "En contact"@fr ,
                             "Limitrophe"@fr ;
               skos:definition "Relation entre repères définissant que le locatum est en contact avec le relatum"@fr,
                               "Relation between landmarks defining that the locatum touches the relatum"@en ,
                               "Relation entre repères définissant que le locatum touche le relatum"@fr ;
               skos:inScheme :AdressSegmentList ;
               skos:prefLabel "Touche"@fr ,
                              "Touches"@en .


###  http://rdf.geohistoricaldata.org/id/codes/address/landmarkRelationType/Within
lrtype:Within rdf:type owl:NamedIndividual ,
                       :LandmarkRelationType ,
                       skos:Concept ;
              skos:altLabel "À l'intérieur"@fr ;
              skos:definition "Relation entre repères définissant que le locatum est situé dans le relatum"@fr ,
                              "Relation entre repères entre des repères définissant que le locatum est dans un relatum"@fr,
                              "Relation between landmarks defining that the locatum is within the relatum"@en ;
              skos:inScheme :AdressSegmentList ,
                            :LandmarkRelationList ;
              skos:prefLabel "Dans"@fr ,
                             "Within"@en .

###  http://rdf.geohistoricaldata.org/id/codes/address/landmarkRelationType/StartsAt
lrtype:StartsAt rdf:type owl:NamedIndividual ,
                      :LandmarkRelationType ,
                      skos:Concept ;
             skos:altLabel "Commence à"@fr ;
             skos:definition "Relation entre repères définissant que le locatum (un repère linéaire) commence au niveau du relatum"@fr, "Relation between landmarks defining that the locatum begins at the relatum"@en ;
             skos:inScheme :AdressSegmentList ,
                           :LandmarkRelationList ;
             skos:prefLabel "Commence à"@fr ,
                            "Starts at"@en .

###  http://rdf.geohistoricaldata.org/id/codes/address/landmarkRelationType/EndsAt
lrtype:EndsAt rdf:type owl:NamedIndividual ,
                      :LandmarkRelationType ,
                      skos:Concept ;
             skos:altLabel "Commence à"@fr ;
             skos:definition "Relation entre repères définissant que le locatum (un repère linéaire) termine au niveau du relatum"@fr, "Relation between landmarks defining that the locatum ends at the relatum"@en ;
             skos:inScheme :AdressSegmentList ,
                           :LandmarkRelationList ;
             skos:prefLabel "Termine à"@fr ,
                            "Ends at"@en .

###  http://rdf.geohistoricaldata.org/id/codes/address/landmarkType/AdministrativeUnity
ltype:AdministrativeUnity rdf:type owl:NamedIndividual ,
                                   :LandmarkType ,
                                   skos:Concept ;
                          skos:definition "Zone résultant d'un découpage administratif (quatier, commune, pays...)"@fr, "Area resulting from an administrative division (district, municipality, country...)"@en ;
                          skos:inScheme :LandmarkList ;
                          skos:prefLabel "Administrative unity"@en ,
                                         "Unité administrative"@fr .

###  http://rdf.geohistoricaldata.org/id/codes/address/landmarkType/PostalCodeArea
ltype:PostalCodeArea rdf:type owl:NamedIndividual ,
                                  :LandmarkType ,
                                  skos:Concept ;
                         skos:definition "Zone postale définie par un code"@fr, "Postal area defined by a code"@en ;
                         skos:inScheme :LandmarkList ;
                         skos:prefLabel "Postal area"@en ,
                                        "Zone postale"@fr .

###  http://rdf.geohistoricaldata.org/id/codes/address/landmarkType/Municipality
ltype:Municipality rdf:type owl:NamedIndividual ,
                    :LandmarkType ,
                    skos:Concept ;
           skos:altLabel "City"@en ,
                         "Town"@en ,
                         "Ville"@fr ;
           skos:broader ltype:AdministrativeUnity ;
           skos:definition "Entité administrative décrivant une ville, une commune"@fr, "Administrative entity describing a city, town or commune"@en ;
           skos:inScheme :LandmarkList ;
           skos:prefLabel "Municipality"@en ,
                          "Commune"@fr .


###  http://rdf.geohistoricaldata.org/id/codes/address/landmarkType/Country
ltype:Country rdf:type owl:NamedIndividual ,
                       :LandmarkType ,
                       skos:Concept ;
              skos:altLabel "State"@en ,
                            "État"@fr ;
              skos:broader ltype:AdministrativeUnity ;
              skos:definition "Entité administrative décrivant un État, un pays"@fr, "Administrative entity describing a state or country"@en ;
              skos:inScheme :LandmarkList ;
              skos:prefLabel "Country"@en ,
                             "Pays"@fr .


###  http://rdf.geohistoricaldata.org/id/codes/address/landmarkType/District
ltype:District rdf:type owl:NamedIndividual ,
                        :LandmarkType ,
                        skos:Concept ;
               skos:altLabel "Hameau"@fr ,
                             "Neighborhood"@en ,
                             "Quarter"@en ;
               skos:broader ltype:AdministrativeUnity ;
               skos:definition "Entité administrative décrivant un quartier"@fr, "Administrative entity describing a district"@en ;
               skos:inScheme :LandmarkList ;
               skos:prefLabel "District"@en ,
                              "Quartier"@fr .


###  http://rdf.geohistoricaldata.org/id/codes/address/landmarkType/DistrictNumber
ltype:DistrictNumber rdf:type owl:NamedIndividual ,
                              :LandmarkType ,
                              skos:Concept ;
                     skos:broader ltype:HouseNumber ;
                     skos:definition "Numéro d'un bâtiment, d'un immeuble lié à un quartier"@fr ;
                     skos:inScheme :LandmarkList ;
                     skos:prefLabel "District number"@en ,
                                    "Numéro de quartier"@fr .


###  http://rdf.geohistoricaldata.org/id/codes/address/landmarkType/HouseNumber
ltype:HouseNumber rdf:type owl:NamedIndividual ,
                           :LandmarkType ,
                           skos:Concept ;
                  skos:definition "Numéro associé à un repère permettant d'identifier un bâtiment, une entreprise, une personne au sein du repère."@fr,
                                  "Number associated with a landmark used to identify a building, a company or a person within the landmark."@en ;
                  skos:inScheme :LandmarkList ;
                  skos:prefLabel "House number"@en ,
                                 "Numéro de l'habitation"@fr .


###  http://rdf.geohistoricaldata.org/id/codes/address/landmarkType/StreetNumber
ltype:StreetNumber rdf:type owl:NamedIndividual ,
                            :LandmarkType ,
                            skos:Concept ;
                   skos:broader ltype:HouseNumber ;
                   skos:definition "Numéro d'un bâtiment, d'un immeuble lié à une rue"@fr, "Number of a building linked to a street"@en ;
                   skos:inScheme :LandmarkList ;
                   skos:prefLabel "Numéro de rue"@fr ,
                                  "Street number"@en .


###  http://rdf.geohistoricaldata.org/id/codes/address/landmarkType/Structure
ltype:Structure rdf:type owl:NamedIndividual ,
                         :LandmarkType ,
                         skos:Concept ;
                skos:definition "Lieu défini (bâtiment, magasin, maison...)"@fr, "Defined location (building, shop, house, etc.)"@en ;
                skos:inScheme :LandmarkList ;
                skos:prefLabel "Structure"@en ,
                               "Structure"@fr .


###  http://rdf.geohistoricaldata.org/id/codes/address/landmarkType/Thoroughfare
ltype:Thoroughfare rdf:type owl:NamedIndividual ,
                            :LandmarkType ,
                            skos:Concept ;
                   skos:definition "Tout élément relatif à une voie de communication (rue, place, avenue...)"@fr, "Any element relating to a thoroughfare (street, square, avenue, etc.)"@en ;
                   skos:inScheme :LandmarkList ;
                   skos:prefLabel "Thoroughfare"@en ,
                                  "Voie"@fr .


###  http://rdf.geohistoricaldata.org/id/codes/address/landmarkType/Undefined
ltype:Undefined rdf:type owl:NamedIndividual ,
                         :LandmarkType ,
                         skos:Concept ;
                skos:definition "Lieu non défini, inconnu"@fr, "Undefined or unknown place"@en ;
                skos:inScheme :LandmarkList ;
                skos:prefLabel "Non défini"@fr ,
                               "Undefined"@en .


###  http://www.w3.org/2006/time#unitCentury
time:unitCentury rdf:type owl:NamedIndividual ,
                          time:TemporalUnit .


###  http://www.w3.org/2006/time#unitDay
time:unitDay rdf:type owl:NamedIndividual ,
                      time:TemporalUnit .


###  http://www.w3.org/2006/time#unitDecade
time:unitDecade rdf:type owl:NamedIndividual ,
                         time:TemporalUnit .


###  http://www.w3.org/2006/time#unitMonth
time:unitMonth rdf:type owl:NamedIndividual ,
                        time:TemporalUnit .


###  http://www.w3.org/2006/time#unitWeek
time:unitWeek rdf:type owl:NamedIndividual ,
                       time:TemporalUnit .


###  http://www.w3.org/2006/time#unitYear
time:unitYear rdf:type owl:NamedIndividual ,
                       time:TemporalUnit .


###  http://www.wikidata.org/entity/Q181974
<http://www.wikidata.org/entity/Q181974> rdf:type owl:NamedIndividual ,
                                                  time:TRS ;
                                         skos:definition "Système de calendrier de la Révolution française"@fr ;
                                         skos:prefLabel "French Republican calendar"@en ,
                                                        "calendrier républicain"@fr .


###  http://www.wikidata.org/entity/Q1985727
<http://www.wikidata.org/entity/Q1985727> rdf:type owl:NamedIndividual ,
                                                   time:TRS ;
                                          skos:definition "Extension du calendrier grégorien à avant son introduction"@fr ;
                                          skos:prefLabel "calendrier grégorien proleptique"@fr ,
                                                         "proleptic Gregorian calendar"@en .
